feat(*) update changes from HOL_Basic library update

HOTG/Arithmetics/Functions_Restrict.thy
@@ -19,7 +19,10 @@ bundle no_fun_restrict_syntax
 begin
 no_notation fun_restrict ("(_)\<restriction>(\<^bsub>_\<^esub>)" [1000])
 end
-unbundle fun_restrict_syntax
+
+context
+  includes fun_restrict_syntax
+begin
 
 lemma fun_restrict_eq [simp]:
   assumes "P x"
@@ -31,14 +34,16 @@ lemma fun_restrict_eq_if_not [simp]:
   shows "f\<restriction>\<^bsub>P\<^esub> x = undefined"
   using assms unfolding fun_restrict_pred_def by auto
 
+end
 
 overloading
   fun_restrict_set \<equiv> "fun_restrict :: (set \<Rightarrow> 'a) \<Rightarrow> set \<Rightarrow> set \<Rightarrow> 'a"
 begin
-  definition "fun_restrict_set f X \<equiv> f\<restriction>\<^bsub>mem_of X\<^esub> :: set \<Rightarrow> 'a"
+  definition "fun_restrict_set f X \<equiv> fun_restrict f (mem_of X) :: set \<Rightarrow> 'a"
 end
 
-lemma fun_restrict_set_eq_fun_restrict [simp]: "(f :: set \<Rightarrow> 'a)\<restriction>\<^bsub>X\<^esub> = f\<restriction>\<^bsub>mem_of X\<^esub>"
+lemma fun_restrict_set_eq_fun_restrict [simp]:
+  "fun_restrict (f :: set \<Rightarrow> 'a) X = fun_restrict f (mem_of X)"
   unfolding fun_restrict_set_def by auto
 
 
