HOTG/Arithmetics/Transfinite_Recursion.thy
@@ -7,6 +7,6 @@ begin
 
 (*TODO: migrate definition from HOL*)
 axiomatization transrec :: "((set \<Rightarrow> 'a) \<Rightarrow> set \<Rightarrow> 'a) \<Rightarrow> set \<Rightarrow> 'a"
-  where transrec_eq: "transrec f X = f ((transrec f)\<restriction>\<^bsub>X\<^esub>) X"
+  where transrec_eq: "transrec f X = f (fun_restrict (transrec f) X) X"
 
 end
