HOTG/Binary_Relations/Properties/SBinary_Relation_Properties.thy
@@ -14,5 +14,6 @@ theory SBinary_Relation_Properties
     SBinary_Relations_Transitive
 begin
 
+(*TODO Kevin: make all concepts overloadings from constants defined in Transport*)
 
 end
