HOTG/Universes.thy
@@ -29,14 +29,14 @@ lemma
 
 text \<open>Variations on transitivity:\<close>
 
-lemma mem_univ_trans: "A \<in> univ X \<Longrightarrow> x \<in> A \<Longrightarrow> x \<in> univ X"
-  using mem_trans_univ unfolding mem_trans_def by auto
+lemma mem_univ_if_mem_if_mem_univ: "A \<in> univ X \<Longrightarrow> x \<in> A \<Longrightarrow> x \<in> univ X"
+  using mem_trans_closed_univ by blast
 
-lemma mem_univ_trans': "x \<in> X \<Longrightarrow> x \<in> univ X"
-  by (rule mem_univ_trans) auto
+lemma mem_univ_if_mem: "x \<in> X \<Longrightarrow> x \<in> univ X"
+  by (rule mem_univ_if_mem_if_mem_univ) auto
 
 lemma subset_univ_if_mem: "A \<in> univ X \<Longrightarrow> A \<subseteq> univ X"
-  using mem_univ_trans by auto
+  using mem_univ_if_mem_if_mem_univ by auto
 
 lemma empty_mem_univ [iff]: "{} \<in> univ X"
 proof -
@@ -46,7 +46,7 @@ proof -
 qed
 
 lemma subset_univ [iff]: "A \<subseteq> univ A"
-  by (auto intro: mem_univ_trans)
+  by (auto intro: mem_univ_if_mem_if_mem_univ)
 
 lemma univ_closed_upair [intro!]:
   "\<lbrakk>x \<in> univ X; y \<in> univ X\<rbrakk> \<Longrightarrow> upair x y \<in> univ X"
@@ -73,14 +73,14 @@ lemma univ_closed_singleton [intro!]: "x \<in> univ U \<Longrightarrow> {x} \<in
   by auto
 
 lemma bin_union_univ_eq_univ_if_mem: "A \<in> univ U \<Longrightarrow> A \<union> univ U = univ U"
-  by (rule eq_if_subset_if_subset) (auto intro: mem_univ_trans)
+  by (rule eq_if_subset_if_subset) (auto intro: mem_univ_if_mem_if_mem_univ)
 
 lemma univ_closed_dep_pairs [intro!]:
   assumes A_mem_univ: "A \<in> univ U"
   and univ_B_closed: "\<And>x. x \<in> A \<Longrightarrow> B x \<in> univ U"
   shows "\<Sum>x \<in> A. (B x) \<in> univ U"
   unfolding dep_pairs_def using assms
-  by (intro univ_closed_union ZF_closed_repl) (auto intro: mem_univ_trans)
+  by (intro univ_closed_union ZF_closed_repl) (auto intro: mem_univ_if_mem_if_mem_univ)
 
 lemma subset_univ_if_subset_univ_pairs: "X \<subseteq> univ A \<times> univ A \<Longrightarrow> X \<subseteq> univ A"
   by auto
@@ -96,7 +96,7 @@ proof -
   let ?P = "powerset (\<Sum>x \<in> A. B x)"
   have "((x \<in> A) \<rightarrow>s (B x)) \<subseteq> ?P" by auto
   moreover have "?P \<in> univ U" using assms by auto
-  ultimately show ?thesis by (auto intro: mem_univ_trans)
+  ultimately show ?thesis by (auto intro: mem_univ_if_mem_if_mem_univ)
 qed
 
 lemma univ_closed_inl [intro!]: "x \<in> univ A \<Longrightarrow> inl x \<in> univ A"
